examples/Examples/Support/NormalizeMetavars.lean
@@ -5,12 +5,12 @@ private inductive NormMetavarState where
   | none
   /-- Saw the leading '?' -/
   | «?» (iter : String.Iterator)
-  /-- Saw the '?m' -/
-  | «?m» (iter : String.Iterator)
-  /-- Saw the '?m.' -/
-  | «?m.» (iter : String.Iterator)
+  /-- Saw the '?m' or '?u' -/
+  | «?m/u» (ch : Char) (iter : String.Iterator)
+  /-- Saw the '?[mu].' -/
+  | «?m/u.» (ch : Char) (iter : String.Iterator)
   /-- Saw one or more digits - '?m.[0-9]+' -/
-  | «?m.[0-9]+» (iter : String.Iterator)
+  | «?m/u.[0-9]+» (ch : Char) (iter : String.Iterator)
 
 /--
 Consistently rewrite all substrings that look like automatic metavariables (e.g "?m.123") so
@@ -32,35 +32,40 @@ def normalizeMetavars (str : String) : String := Id.run do
       else
         out := out.push c
     | .«?» i =>
-      state := if c == 'm' then .«?m» i else .none
-    | .«?m» i =>
-      state := if c == '.' then .«?m.» i else .none
-    | .«?m.» i =>
-      state := if c.isDigit then .«?m.[0-9]+» i else .none
-    | .«?m.[0-9]+» i =>
+      if c == 'm' || c == 'u' then
+        state := .«?m/u» c i
+      else
+        state := .none
+        out := out.push '?'
+        out := out.push c
+    | .«?m/u» c' i =>
+      state := if c == '.' then .«?m/u.» c' i else .none
+    | .«?m/u.» c' i =>
+      state := if c.isDigit then .«?m/u.[0-9]+» c' i else .none
+    | .«?m/u.[0-9]+» c' i =>
       unless c.isDigit do
         state := .none
         let mvarStr := i.extract iter
         match nums[mvarStr]? with
         | none =>
           nums := nums.insert mvarStr gensymCounter
-          out := out ++ s!"?m.{gensymCounter}"
+          out := out ++ s!"?{c'}.{gensymCounter}"
           gensymCounter := gensymCounter + 1
-        | some s => out := out ++ s!"?m.{s}"
+        | some s => out := out ++ s!"?{c'}.{s}"
         out := out.push c
 
     iter := iter.next
 
   match state with
-  | .«?m.[0-9]+» i =>
+  | .«?m/u.[0-9]+» c' i =>
     let mvarStr := i.extract iter
     match nums[mvarStr]? with
     | none =>
       nums := nums.insert mvarStr gensymCounter
-      out := out ++ s!"?m.{gensymCounter}"
+      out := out ++ s!"?{c'}.{gensymCounter}"
       gensymCounter := gensymCounter + 1
-    | some s => out := out ++ s!"?m.{s}"
-  | .«?» i  | .«?m» i | .«?m.» i =>
+    | some s => out := out ++ s!"?{c'}.{s}"
+  | .«?» i  | .«?m/u» _c' i | .«?m/u.» _c' i =>
     out := out ++ i.extract iter
   | .none => pure ()
 
@@ -69,6 +74,14 @@ def normalizeMetavars (str : String) : String := Id.run do
 /-- info: "List ?m.1" -/
 #guard_msgs in
 #eval normalizeMetavars "List ?m.9783"
+
+/-- info: "Type ?u.1" -/
+#guard_msgs in
+#eval normalizeMetavars "Type ?u.9783"
+
+/-- info: "Type ?x.9783" -/
+#guard_msgs in
+#eval normalizeMetavars "Type ?x.9783"
 
 /-- info: "List ?m.1 " -/
 #guard_msgs in
@@ -107,7 +120,7 @@ xs : List ?m.1034
 elem : x ∈ xs
 ⊢ xs.length > 0"##
 
-/-- info: "x : ?m.1\nα : Type .1234\nxs : List ?m.2\nelem : x ∈ xs\n⊢ xs.length > 0" -/
+/-- info: "x : ?m.1\nα : Type ?u.2\nxs : List ?m.3\nelem : x ∈ xs\n⊢ xs.length > 0" -/
 #guard_msgs in
 #eval normalizeMetavars
   r##"x : ?m.1035
