functional-programming-lean/src/dependent-types.md
@@ -5,11 +5,11 @@ Types and programs have different grammars and they are used at different times.
 Types are typically used at compile time, to check that a program obeys certain invariants.
 Programs are used at run time, to actually perform computations.
 When the two interact, it is usually in the form of a type-case operator like an "instance-of" check or a casting operator that provides the type checker with information that was otherwise unavailable, to be verified at run time.
-In other words, the interaction consists of types being inserted into the world of programs, gaining some limited run-time meaning.
+In other words, the interaction consists of types being inserted into the world of programs, where they gain some limited run-time meaning.
 
 Lean does not impose this strict separation.
 In Lean, programs may compute types and types may contain programs.
-Placing programs in types allows their full computation power to be used at compile time, and the ability to return types from functions makes types into first-class participants in the programming process.
+Placing programs in types allows their full computational power to be used at compile time, and the ability to return types from functions makes types into first-class participants in the programming process.
 
 _Dependent types_ are types that contain non-type expressions.
 A common source of dependent types is a named argument to a function.
